engine/lib/phases/phase_functionalize_loops.ml
@@ -32,6 +32,65 @@ struct
       include Features.SUBTYPE.Id
     end
 
+    module ItExpr = struct
+      open A
+
+      type kind =
+        | Range of { min : expr; max : expr }
+        (* | Enumerate of t *)
+        (* | Zip of t * t *)
+        (* | ChunksExact of { it : t; size : expr } *)
+        | Indexable of expr  (** a slice, an array *)
+
+      and t = { kind : kind; typ : ty }
+
+      module Expect = struct
+        include UA.Expect
+
+        let ( <|> ) (type a b) (f : a -> b option) (g : a -> b option) x =
+          match f x with Some r -> Some r | None -> g x
+
+        let any_ref (typ : ty) : ty option =
+          match typ with TRef { typ; _ } -> Some typ | _ -> None
+
+        let array (typ : ty) : ty option =
+          match typ with TArray { typ; _ } -> Some typ | _ -> None
+
+        let slice (typ : ty) : ty option =
+          match typ with TSlice { ty; _ } -> Some ty | _ -> None
+
+        let into_iter : expr -> expr option =
+         fun e ->
+          concrete_app1 Core__iter__traits__collect__IntoIterator__into_iter e
+
+        let concrete_app_n (f : Concrete_ident.name) (e : expr) :
+            expr list option =
+          match e.e with
+          | App { f = { e = GlobalVar (`Concrete f'); _ }; args; _ }
+            when Concrete_ident.eq_name f f' ->
+              Some args
+          | _ -> None
+
+        let concrete_app2 (f : Concrete_ident.name) (e : expr) :
+            (expr * expr) option =
+          match concrete_app_n f e with
+          | Some [ x; y ] -> Some (x, y)
+          | _ -> None
+
+        let indexable (e : expr) : t option =
+          let* e = into_iter e in
+          let* typ =
+            any_ref e.typ |> Option.value ~default:e.typ |> (array <|> slice)
+          in
+          Some { kind = Indexable e; typ }
+
+        let range (e : expr) : t option =
+          let* e = into_iter e in
+          let* min, max = concrete_app2 Core__ops__range__Range e in
+          Some { kind = Range { min; max }; typ = min.typ }
+      end
+    end
+
     [%%inline_defs dmutability]
 
     let rec dexpr_unwrapped (expr : A.expr) : B.expr =
@@ -62,8 +121,30 @@ struct
             Core__iter__traits__iterator__Iterator__fold
             [ it; dexpr init; fn ]
             span (dty span expr.typ)
-      | Loop { state = None; _ } ->
-          Error.unimplemented ~details:"Loop without mutation?" span
+      | Loop
+          {
+            body;
+            kind = ForIndexLoop { start; end_; var = var, var_typ, var_span; _ };
+            state = None;
+            _;
+          } ->
+          let var_typ = dty var_span var_typ in
+          let body = dexpr body in
+          let fn : B.expr =
+            let e : B.expr' =
+              let arg = UB.make_var_pat var var_typ var_span in
+              Closure { params = [ arg ]; body; captures = [] }
+            in
+            let typ = B.TArrow ([ var_typ ], body.typ) in
+            { e; typ; span = body.span }
+          in
+          UB.call ~kind:(AssociatedItem Value) Rust_primitives__hax__for_loop
+            [ dexpr start; dexpr end_; fn ]
+            span (dty span expr.typ)
+      | Loop { state = None; _ } as hey ->
+          Stdio.prerr_endline @@ ">>>" ^ [%show: A.expr'] hey;
+            Error.unimplemented
+            ~details:"Loop without mutation?HERE" span
       | Loop _ ->
           Error.unimplemented
             ~details:"Only for loop are being functionalized for now" span
