engine/lib/phases/phase_local_mutation.ml
@@ -4,14 +4,12 @@ open Side_effect_utils
 
 module%inlined_contents Make
     (F : Features.T
-           with type mutable_reference = Features.Off.mutable_reference
-            and type mutable_pointer = Features.Off.mutable_pointer
+           with type mutable_pointer = Features.Off.mutable_pointer
             and type raw_pointer = Features.Off.raw_pointer
             and type arbitrary_lhs = Features.Off.arbitrary_lhs
             and type nontrivial_lhs = Features.Off.nontrivial_lhs
             and type monadic_action = Features.Off.monadic_action
-            and type monadic_binding = Features.Off.monadic_binding
-            and type for_index_loop = Features.Off.for_index_loop) =
+            and type monadic_binding = Features.Off.monadic_binding) =
 struct
   open Ast
   module FA = F
