engine/lib/phases/phase_local_mutation.mli
@@ -2,14 +2,12 @@ open! Prelude
 
 module Make
     (F : Features.T
-           with type mutable_reference = Features.Off.mutable_reference
-            and type mutable_pointer = Features.Off.mutable_pointer
+           with type mutable_pointer = Features.Off.mutable_pointer
             and type raw_pointer = Features.Off.raw_pointer
             and type arbitrary_lhs = Features.Off.arbitrary_lhs
             and type nontrivial_lhs = Features.Off.nontrivial_lhs
             and type monadic_action = Features.Off.monadic_action
-            and type monadic_binding = Features.Off.monadic_binding
-            and type for_index_loop = Features.Off.for_index_loop) : sig
+            and type monadic_binding = Features.Off.monadic_binding) : sig
   include module type of struct
     module FA = F
 
