proof-libs/fstar/rust_primitives/Rust_primitives.fst
@@ -3,24 +3,52 @@ module Rust_primitives
 include Rust_primitives.Integers
 include Rust_primitives.Arrays
 
+inline_for_extraction
 class cast_tc a b = {
   cast: a -> b; 
 }
 
 /// Rust's casts operations on integers are non-panicking
+inline_for_extraction
 instance cast_tc_integers (t:inttype) (t':inttype)
   : cast_tc (int_t t) (int_t t')
   = { cast = (fun x -> Rust_primitives.Integers.cast_mod #t #t' x) }
 
+module B = LowStar.Buffer
+module HS = FStar.HyperStack
+module HST = FStar.HyperStack.ST
+
+inline_for_extraction
 class unsize_tc source = {
   output: Type;
-  unsize: source -> output;
+  unsize: source -> output
 }
 
+inline_for_extraction
 instance array_to_slice_unsize t n: unsize_tc (t_Array t n) = {
   output = t_Slice t;
   unsize = (fun (arr: t_Array t n) -> 
-            arr <: t_Slice t);
+    Some {buffer = arr; len = n}
+  );
 }
 
+open FStar.HyperStack
+open FStar.HyperStack.ST
+
+// open Lib.IntTypes
+
+inline_for_extraction
+val f_for_loop: #n: inttype ->
+    start: int_t n
+  -> finish: int_t n {v finish >= v start}
+  -> f:(i:int_t n (*{v start <= v i /\ v i < v finish}*) -> St unit) ->
+  St unit
+let f_for_loop #n start0 finish0 f = 
+    let start  = Rust_primitives.Integers.cast_mod start0  in
+    let finish = Rust_primitives.Integers.cast_mod finish0 in
+    admitP (v finish0 >= v start0 ==> v finish >= v start);
+    Lib.Loops.for
+        start finish
+        (fun _ _ -> True)
+        (fun i -> f (Rust_primitives.Integers.cast_mod i); admit ())
 
