proof-libs/fstar/core/Core.Array.fst
@@ -1,10 +1,16 @@
 module Core.Array
 open Rust_primitives
 
+
+open LowStar.BufferOps
+module B = LowStar.Buffer
+module HS = FStar.HyperStack
+module HST = FStar.HyperStack.ST
+
+
 type t_TryFromSliceError = | TryFromSliceError
 
-let impl_23__map n (arr: t_Array 'a n) (f: 'a -> 'b): t_Array 'b n 
-  = map_array arr f
+// let impl_23__map n (arr: t_Array 'a n) (f: 'a -> 'b): t_Array 'b n 
+//   = map_array arr f
 
-let impl_23__as_slice len (arr: t_Array 'a len): t_Slice 'a = arr
-
+let impl_23__as_slice len (arr: t_Array 'a len): HST.St (t_Slice 'a) = admit ()
