proof-libs/fstar/core/Core.Ops.fst
@@ -1,6 +1,11 @@
 module Core.Ops
 open Rust_primitives
 
+open LowStar.BufferOps
+module B = LowStar.Buffer
+module HS = FStar.HyperStack
+module HST = FStar.HyperStack.ST
+
 // class add_tc self rhs = {
 //   output: Type;
 //   in_bounds: self -> rhs -> Type0;
@@ -22,6 +27,6 @@ instance negation_for_bool: negation_tc bool = {
 open Core.Ops.Index
 
 let ( .[] ) #self #idx {| inst: t_Index self idx |}
-  : s:self -> i:idx{in_range s i} -> inst.f_Output
+  : s:self -> i:idx{in_range s i} -> HST.St inst.f_Output
   = f_index
 
