proof-libs/fstar/rust_primitives/Rust_primitives.Hax.fst
@@ -6,14 +6,20 @@ open Rust_primitives.Arrays
 type t_Never = False
 let never_to_any #t: t_Never -> t = (fun _ -> match () with)
 
-let repeat (x: 'a) (len: usize): t_Array 'a len = 
-  FStar.Seq.create (v len) x
+open LowStar.BufferOps
+module B = LowStar.Buffer
+module HS = FStar.HyperStack
+module HST = FStar.HyperStack.ST
+
+let repeat (x: 'a) (len: usize {v len > 0}): HST.StackInline (t_Array 'a len) (fun _ -> True) (fun _ _ _ -> True) = 
+  B.alloca x len
 
 open Core.Ops.Index
+
 class update_at_tc self idx = {
   [@@@FStar.Tactics.Typeclasses.tcinstance]
   super_index: t_Index self idx;
-  update_at: s: self -> i: idx {in_range s i} -> super_index.f_Output -> self;
+  update_at: s: self -> i: idx {in_range s i} -> super_index.f_Output -> HST.St unit;
 }
 
 open Core.Slice
@@ -21,20 +27,30 @@ open Core.Slice
 instance impl__index t l n: t_Index (t_Array t l) (int_t n)
   = { f_Output = t;
       in_range = (fun (s: t_Array t l) (i: int_t n) -> v i >= 0 && v i < v l);
-      f_index = (fun s i -> Seq.index s (v i));
+      f_index = (fun s i -> admit (); s.(i));
     }
 
 instance update_at_tc_array t l n: update_at_tc (t_Array t l) (int_t n) = {
   super_index = FStar.Tactics.Typeclasses.solve <: t_Index (t_Array t l) (int_t n);
-  update_at = (fun arr i x -> FStar.Seq.upd arr (v i) x);
+  update_at = (fun arr i x -> 
+            admit ();
+            arr.(i) <- x
+    );
+}
+
+instance update_at_tc_slice t n: update_at_tc (t_Slice t) (int_t n) = {
+  super_index = FStar.Tactics.Typeclasses.solve <: t_Index (t_Slice t) (int_t n);
+  update_at = (fun arr i x -> 
+            admit ()
+            // arr.(i) <- x
+    );
 }
 
 let (.[]<-) #self #idx {| update_at_tc self idx |} (s: self) (i: idx {in_range s i})
   = update_at s i
 
+inline_for_extraction
 let array_of_list #t = Rust_primitives.Arrays.of_list #t
-
-
 
 // class index self idx = {
 //   [@@@FStar.Tactics.Typeclasses.no_method]
@@ -56,5 +72,6 @@ let array_of_list #t = Rust_primitives.Arrays.of_list #t
 //   in_range = (fun (_:array t l) (idx: int_t n) -> v idx >= 0 && v idx < v l);
 //   (.[]) = (fun (x:array t l) idx -> Seq.index x (v idx));
 // }
+
 
 
